(WIP) Define combinational-only semantics

vera/VerilogSemantics.v
@@ -8,8 +8,9 @@ From Coq Require FMapFacts.
 From Coq Require Import List.
 From Coq Require Import ssreflect.
 From Coq Require Import Relations.
+From Coq Require Import Structures.Equalities.
 
-From vera Require Import Verilog.
+From vera Require Verilog.
 From vera Require Import Common.
 
 From nbits Require Import NBits.
@@ -27,373 +28,137 @@ Local Open Scope monad_scope.
 
 Set Bullet Behavior "Strict Subproofs".
 
-Definition Process := TypedVerilog.module_item.
+Module CombinationalOnly(VType: DecidableType).
+  Module Verilog := Verilog.MkVerilog(VType).
 
-Definition PendingProcesses := list Process.
+  Definition Process := Verilog.module_item.
 
-Record VerilogState :=
-  MkVerilogState
-    { regState : StrMap.t bits
-    ; nbaValues : StrMap.t bits
-    ; pendingProcesses : NameMap.t Process
-    }
-.
+  Record VerilogState :=
+    MkVerilogState
+      { regState : StrMap.t bits
+      ; pendingProcesses : list Process
+      }
+  .
 
-Definition set_reg (name : string) (value : bits) (st : VerilogState) : VerilogState :=
-  {| regState := StrMap.add name value (regState st)
-  ; nbaValues := nbaValues st
-  ; pendingProcesses := pendingProcesses st
-  |}
-.
+  Definition set_reg (name : string) (value : bits) (st : VerilogState) : VerilogState :=
+    {| regState := StrMap.add name value (regState st)
+    ; pendingProcesses := pendingProcesses st
+    |}
+  .
 
-Definition set_nba (name : string) (value : bits) (st : VerilogState) : VerilogState :=
-  {| regState := regState st
-  ; nbaValues := StrMap.add name value (nbaValues st)
-  ; pendingProcesses := pendingProcesses st
-  |}
-.
+  Definition pop_pending_process (st : VerilogState) : VerilogState :=
+    {| regState := regState st
+    ; pendingProcesses := tail (pendingProcesses st)
+    |}
+  .
 
-Definition remove_process (name : name) (st : VerilogState) : VerilogState :=
-  {| regState := regState st
-  ; nbaValues := nbaValues st
-  ; pendingProcesses := NameMap.remove name (pendingProcesses st)
-  |}
-.
+  Equations
+    eval_op (op : Verilog.op) (lhs rhs : bits) (width_match : size lhs = size rhs) : bits :=
+    eval_op Verilog.BinaryPlus lhs rhs prf := lhs +# rhs;
+    eval_op _ lhs rhs prf := _
+  .
+  Admit Obligations.
 
-Equations
-  eval_op (op : Verilog.op) (lhs rhs : bits) (width_match : size lhs = size rhs) : bits :=
-  eval_op Verilog.BinaryPlus lhs rhs prf := lhs +# rhs;
-  eval_op _ lhs rhs prf := _
-.
-Admit Obligations.
+  Equations
+    eval_expr : VerilogState -> Verilog.expression -> option bits :=
+    eval_expr st (Verilog.BinaryOp _ op lhs rhs) :=
+      lhs__val <- eval_expr st lhs ;;
+      rhs__val <- eval_expr st rhs ;;
+      match eq_dec (size lhs__val) (size rhs__val) with
+      | left prf => ret (eval_op op lhs__val rhs__val _)
+      | right _ => None
+      end;
+    eval_expr st (Verilog.Conditional cond tBranch fBranch) :=
+      cond__val <- eval_expr st cond ;;
+      tBranch__val <- eval_expr st tBranch ;;
+      fBranch__val <- eval_expr st fBranch ;;
+      match (eq_dec (size tBranch__val) (size fBranch__val)), (eq_dec cond__val ((size cond__val)-bits of 0)) with
+      | left size_ok, left cond_zero => ret fBranch__val
+      | left size_ok, right cond_not_zero => ret tBranch__val
+      | right _, _ => None
+      end;
+    eval_expr st (Verilog.BitSelect vec idx) :=
+      vec__val <- eval_expr st vec ;;
+      idx__val <- eval_expr st idx ;;
+      ret [ nth false vec__val (to_nat idx__val) ];
+    eval_expr st (Verilog.Annotation _ expr) := eval_expr st expr ;
+    eval_expr st (Verilog.IntegerLiteral val) := Some val;
+    eval_expr st (Verilog.NamedExpression _ name) := StrMap.find name (regState st)
+  .
 
-Require Import Psatz.
+  Equations
+    exec_statement (st : VerilogState) (stmt : Verilog.statement) : option VerilogState by struct :=
+    exec_statement st (Verilog.Block stmts) := exec_statements st stmts ;
+    exec_statement st (Verilog.If cond trueBranch falseBranch) :=
+      condVal <- eval_expr st cond ;;
+      if (to_nat condVal) =? 0
+      then exec_statement st falseBranch
+      else exec_statement st trueBranch
+    ;
+    exec_statement st (Verilog.BlockingAssign (Verilog.NamedExpression _ name) rhs) :=
+      rhs__val <- eval_expr st rhs ;;
+      Some (set_reg name rhs__val st)
+    ;
+    exec_statement st (Verilog.BlockingAssign lhs rhs) :=
+      None;
+    exec_statement st (Verilog.NonBlockingAssign lhs rhs) :=
+      None;
+  where exec_statements (st : VerilogState) (stmts : list Verilog.statement) : option VerilogState :=
+    exec_statements st [] := Some st;
+    exec_statements st (hd :: tl) :=
+      st' <- exec_statement st hd ;;
+      exec_statements st' tl;
+  .
 
-Equations
-  eval_expr : VerilogState -> TypedVerilog.expression -> option bits :=
-  eval_expr st (TypedVerilog.BinaryOp _ op lhs rhs) :=
-    lhs__val <- eval_expr st lhs ;;
-    rhs__val <- eval_expr st rhs ;;
-    match eq_dec (size lhs__val) (size rhs__val) with
-    | left prf => ret (eval_op op lhs__val rhs__val _)
-    | right _ => None
-    end;
-  eval_expr st (TypedVerilog.Conditional cond tBranch fBranch) :=
-    cond__val <- eval_expr st cond ;;
-    tBranch__val <- eval_expr st tBranch ;;
-    fBranch__val <- eval_expr st fBranch ;;
-    match (eq_dec (size tBranch__val) (size fBranch__val)), (eq_dec cond__val ((size cond__val)-bits of 0)) with
-    | left size_ok, left cond_zero => ret fBranch__val
-    | left size_ok, right cond_not_zero => ret tBranch__val
-    | right _, _ => None
-    end;
-  eval_expr st (TypedVerilog.BitSelect vec idx) :=
-    vec__val <- eval_expr st vec ;;
-    idx__val <- eval_expr st idx ;;
-    ret [ nth false vec__val (to_nat idx__val) ];
-  eval_expr st (TypedVerilog.Conversion from_type to_type expr) :=
-    val <- eval_expr st expr;;
-    ret (if size val <? to_type
-         then zext to_type val
-         else low to_type val)
-  ;
-  eval_expr st (TypedVerilog.IntegerLiteral val) := Some val;
-  eval_expr st (TypedVerilog.NamedExpression _ name) := StrMap.find name (regState st)
-.
+  Lemma exec_statement_procs : forall st1 stmt st2,
+      exec_statement st1 stmt = Some st2 ->
+      pendingProcesses st1 = pendingProcesses st2
+  .
+  Proof.
+    refine (fst (exec_statement_elim
+                   (fun st1 stmt mSt2 => forall st2, mSt2 = Some st2 -> pendingProcesses st1 = pendingProcesses st2)
+                   (fun st1 stmts mSt2 => forall st2, mSt2 = Some st2 -> pendingProcesses st1 = pendingProcesses st2)
+                   _ _ _ _ _ _ _ _ _ _ _ )); intros; auto; try discriminate.
+    - inversion H; destruct (eval_expr st rhs); try discriminate; clear H.
+      inversion H1; clear H1.
+      reflexivity.
+    - inversion H1; destruct (eval_expr st cond); try discriminate; clear H1.
+      destruct (to_nat b =? 0); auto.
+    - inversion H. reflexivity.
+    - inversion H1; clear H1.
+      destruct (exec_statement st hd) eqn:E; try discriminate.
+      transitivity (pendingProcesses v); eauto.
+  Qed.
 
-Equations
-  exec_statement (st : VerilogState) (stmt : TypedVerilog.Statement) : option VerilogState by struct :=
-  exec_statement st (TypedVerilog.Block stmts) := exec_statements st stmts ;
-  exec_statement st (TypedVerilog.If cond trueBranch falseBranch) :=
-    condVal <- eval_expr st cond ;;
-    if (to_nat condVal) =? 0
-    then exec_statement st falseBranch
-    else exec_statement st trueBranch
-  ;
-  exec_statement st (TypedVerilog.BlockingAssign (TypedVerilog.NamedExpression _ name) rhs) :=
-    rhs__val <- eval_expr st rhs ;;
-    Some (set_reg name rhs__val st)
-  ;
-  exec_statement st (TypedVerilog.BlockingAssign lhs rhs) :=
-    None;
-  exec_statement st (TypedVerilog.NonBlockingAssign (TypedVerilog.NamedExpression _ name) rhs) :=
-    rhs__val <- eval_expr st rhs ;;
-    Some (set_nba name rhs__val st)
-  ;
-  exec_statement st (TypedVerilog.NonBlockingAssign lhs rhs) :=
-    None;
-where exec_statements (st : VerilogState) (stmts : list TypedVerilog.Statement) : option VerilogState :=
-  exec_statements st [] := Some st;
-  exec_statements st (hd :: tl) :=
-    st' <- exec_statement st hd ;;
-    exec_statements st' tl;
-.
+  Definition least_element {A} (m : NameMap.t A) : option (name * A) :=
+    List.hd_error (NameMap.elements m).
 
-Equations
-  exec_module_item : VerilogState -> TypedVerilog.module_item -> option VerilogState :=
-  exec_module_item st (TypedVerilog.Initial _) :=
-    Some st;
-  exec_module_item st (TypedVerilog.AlwaysFF stmt) :=
-    exec_statement st stmt;
-  exec_module_item st (TypedVerilog.AlwaysComb stmt ) :=
-    exec_statement st stmt; (* TODO: Do we need to handle always_comb differently? *)
-.
+  Equations
+    exec_module_item : VerilogState -> Verilog.module_item -> option VerilogState :=
+    exec_module_item st (Verilog.Initial _) :=
+      Some st;
+    exec_module_item st (Verilog.AlwaysFF stmt) :=
+      None; (* always_ff is not allowed *)
+    exec_module_item st (Verilog.AlwaysComb stmt ) :=
+      exec_statement st stmt;
+  .
 
-Lemma exec_statement_procs : forall st1 stmt st2,
-    exec_statement st1 stmt = Some st2 ->
-    pendingProcesses st1 = pendingProcesses st2
-.
-Proof.
-  refine (fst (exec_statement_elim
-                 (fun st1 stmt mSt2 => forall st2, mSt2 = Some st2 -> pendingProcesses st1 = pendingProcesses st2)
-                 (fun st1 stmts mSt2 => forall st2, mSt2 = Some st2 -> pendingProcesses st1 = pendingProcesses st2)
-                 _ _ _ _ _ _ _ _ _ _ _ _ _ _ _ _)); intros; auto; try discriminate.
-  - inversion H; destruct (eval_expr st rhs); try discriminate; clear H.
-    inversion H1; clear H1.
-    reflexivity.
-  - inversion H; destruct (eval_expr st rhs); try discriminate; clear H.
-    inversion H1; clear H1.
-    reflexivity.
-  - inversion H1; destruct (eval_expr st cond); try discriminate; clear H1.
-    destruct (to_nat b =? 0); auto.
-  - inversion H. reflexivity.
-  - inversion H1; clear H1.
-    destruct (exec_statement st hd) eqn:E; try discriminate.
-    transitivity (pendingProcesses v); eauto.
-Qed.
+  Equations step : VerilogState -> option VerilogState :=
+    step (MkVerilogState reg []) := None;
+    step (MkVerilogState reg (p :: ps)) := exec_module_item (MkVerilogState reg ps) p.
 
-Lemma exec_module_item_procs : forall st1 st2 mi,
-    exec_module_item st1 mi = Some st2 ->
-    pendingProcesses st1 = pendingProcesses st2
-.
-Proof.
-  intros * H.
-  funelim (exec_module_item st1 mi); simp exec_module_item in *.
-  - eauto using exec_statement_procs.
-  - eauto using exec_statement_procs.
-  - inversion H. subst. reflexivity.
-Qed.
+  Definition blocked (st : VerilogState) : Prop :=
+    step st = None.
 
-Definition least_element {A} (m : NameMap.t A) : option (name * A) :=
-  List.hd_error (NameMap.elements m).
+  Definition final (st : VerilogState) : Prop :=
+    pendingProcesses st = [].
 
-Definition flush_nonblocking (st : VerilogState) : VerilogState :=
-  {|
-    regState := StrMap.map2 opt_or (nbaValues st) (regState st);
-    nbaValues := StrMap.empty bits;
-    pendingProcesses := pendingProcesses st
-  |}
-.
-
-Inductive step_ndet (st1 st2 : VerilogState) : Prop :=
-| step_ndet_exec_process
-    (p_name : name)
-    (p : Process)
-    (p_pending : NameMap.MapsTo p_name p (pendingProcesses st1))
-    (p_exec : exec_module_item (remove_process p_name st1) p = Some st2)
-    (p_removed : pendingProcesses st2 = NameMap.remove p_name (pendingProcesses st1))
-| step_ndet_flush_nonblocking
-    (no_processes_pending : NameMap.Empty (pendingProcesses st1))
-    (nba_pending : ~ StrMap.Empty (nbaValues st1))
-    (flushed : st2 = flush_nonblocking st1)
-.
-
-Definition ndet_blocked (st : VerilogState) : Prop :=
-  ~ exists st', step_ndet st st'.
-
-Definition ndet_final (st : VerilogState) : Prop :=
-  NameMap.Empty (pendingProcesses st) /\ StrMap.Empty (nbaValues st).
-
-Lemma ndet_final_blocked_iff (st : VerilogState) : ndet_final st -> ndet_blocked st.
-Proof.
-  intros [Hprocs Hnbas] [st' Hstep].
-  destruct Hstep.
-  - eapply Hprocs. eauto.
-  - contradiction.
-Qed.
-
-Definition multistep_ndet : VerilogState -> VerilogState -> Prop :=
-  clos_refl_trans VerilogState step_ndet.
-
-Definition evaluate_ndet (st1 st2 : VerilogState) : Prop :=
-  multistep_ndet st1 st2 /\ ndet_final st2.
-
-Inductive step_sequential (st1 st2 : VerilogState) :=
-| step_sequential_exec_process
-    (p_name : name)
-    (p : Process)
-    (p_first : least_element (pendingProcesses st1) = Some (p_name, p))
-    (p_exec : exec_module_item (remove_process p_name st1) p = Some st2)
-.
-
-Equations stmt_driven_signals : TypedVerilog.Statement -> StrSet.t :=
-  stmt_driven_signals (TypedVerilog.Block body) :=
-    List.fold_left StrSet.union (List.map stmt_driven_signals body) StrSet.empty;
-  stmt_driven_signals (TypedVerilog.BlockingAssign (TypedVerilog.NamedExpression _ n) rhs) :=
-    StrSet.singleton n ;
-  stmt_driven_signals (TypedVerilog.BlockingAssign _ _) :=
-    StrSet.empty;
-  stmt_driven_signals (TypedVerilog.NonBlockingAssign (TypedVerilog.NamedExpression _ n) rhs) :=
-    StrSet.singleton n ;
-  stmt_driven_signals (TypedVerilog.NonBlockingAssign _ _) :=
-    StrSet.empty;
-  stmt_driven_signals (TypedVerilog.If _ trueBranch falseBranch) :=
-    StrSet.union (stmt_driven_signals trueBranch) (stmt_driven_signals falseBranch)
-.
-
-Equations driven_signals : Process -> StrSet.t :=
-  driven_signals (TypedVerilog.AlwaysFF stmts) :=
-    stmt_driven_signals stmts;
-  driven_signals (TypedVerilog.AlwaysComb stmts) :=
-    stmt_driven_signals stmts;
-  driven_signals (TypedVerilog.Initial stmts) :=
-    StrSet.empty
-.
-
-Definition is_combinational (p : Process) : Prop :=
-  match p with
-  | TypedVerilog.AlwaysComb _ => True
-  | _ => False
-  end
-.
-
-Definition no_combinational (st : VerilogState) : Prop :=
-  forall n p, NameMap.MapsTo n p (pendingProcesses st) -> ~ is_combinational p
-.
-
-Definition single_driver (st : VerilogState) :=
-  forall n1 n2 p1 p2,
-    n1 <> n2 ->
-    NameMap.MapsTo n1 p1 (pendingProcesses st) ->
-    NameMap.MapsTo n2 p2 (pendingProcesses st) ->
-    StrSet.Empty (StrSet.inter (driven_signals p1) (driven_signals p2))
-.
-
-(* Invalid, because they are equivalent in the eventual state, not in each individual step *)
-Conjecture ndet_sequential_equivalence:
-  forall (st1 st2 st2': VerilogState),
-    single_driver st1 ->
-    no_combinational st1 ->
-    step_ndet st1 st2 ->
-    step_sequential st1 st2' ->
-    st2 = st2'.
-(* No matter what process we pick for ndet, it will not affect the evaluation of other processes *)
-
-Import VerilogNotations.
-
-Definition nondeterminism1 : TypedVerilog.vmodule :=
-  {|
-    TypedVerilog.modName := "nondeterminism1";
-    TypedVerilog.modPorts := [
-      Verilog.MkPort PortIn "clk";
-      Verilog.MkPort PortOut "a";
-      Verilog.MkPort PortOut "b"
-    ];
-    TypedVerilog.modVariables := [
-      Verilog.MkVariable [1.:0] Verilog.Reg "a";
-      Verilog.MkVariable [1.:0] Verilog.Reg "b"
-    ];
-    TypedVerilog.modBody := [
-      TypedVerilog.AlwaysFF
-        ( TypedVerilog.BlockingAssign
-            (TypedVerilog.NamedExpression 2 "a")
-            (TypedVerilog.BinaryOp
-               2
-               Verilog.BinaryPlus
-               (TypedVerilog.NamedExpression 2 "a")
-               (TypedVerilog.IntegerLiteral (2-bits of 1))));
-      TypedVerilog.AlwaysFF
-        ( TypedVerilog.BlockingAssign
-            (TypedVerilog.NamedExpression 2 "b")
-            (TypedVerilog.NamedExpression 2 "a"))
-    ]
-  |}
-.
-
-Definition initial_state (m : TypedVerilog.vmodule) : VerilogState :=
-  {|
-    regState :=
-      (* TODO: correct initialization of regs *)
-      List.fold_left
-        (fun vars var =>
-           StrMap.add
-             (Verilog.varName var)
-             ((Verilog.vector_declaration_width (Verilog.varVectorDeclaration var))-bits of 0)
-             vars)
-        (TypedVerilog.modVariables m)
-        (StrMap.empty bits);
-    nbaValues := StrMap.empty bits;
-    pendingProcesses :=
-      snd
-        (List.fold_left
-           (fun '(nextName, procs) proc =>
-            (Pos.succ nextName, NameMap.add nextName proc procs))
-           (TypedVerilog.modBody m)
-           (1%positive, NameMap.empty Process))
-  |}
-.
-
-(* Compute (initial_state nondeterminism1). *)
-
-Ltac verilog_exec_tac :=
-  repeat progress
-    (simp exec_module_item exec_statement eval_expr
-     || unfold remove_process, set_reg
-     || simpl).
-
-Ltac verilog_step_process_tac n :=
-  apply rt_step;
-  eapply step_ndet_exec_process with (p_name := n);
-  repeat (try progress verilog_exec_tac; reflexivity).
-
-Ltac maps_to_tac :=
-  apply StrMap.find_mapsto_iff;
-  unfold StrMap.add, StrMap.find;
-  simpl;
-  (reflexivity || f_equal).
-
-Example nondeterminism1_eval1 :
-  exists st,
-    evaluate_ndet (initial_state nondeterminism1) st
-    /\ StrMap.MapsTo "a"%string (2-bits of 1) (regState st)
-    /\ StrMap.MapsTo "b"%string (2-bits of 1) (regState st)
-.
-Proof.
-  unfold evaluate_ndet.
-  eexists.
-  repeat split.
-  {
-    unfold nondeterminism1, initial_state; simpl.
-    eapply rt_trans.
-    - verilog_step_process_tac 1%positive.
-    - verilog_step_process_tac 2%positive.
-  }
-  all: simpl; simp eval_op bv_add_truncate.
-  - apply NameMap.is_empty_iff. reflexivity.
-  - apply StrMap.is_empty_iff. reflexivity.
-  - maps_to_tac.
-  - maps_to_tac.
-Qed.
-
-Example nondeterminism1_eval2 :
-  exists st,
-    evaluate_ndet (initial_state nondeterminism1) st
-    /\ StrMap.MapsTo "a"%string (2-bits of 1) (regState st)
-    /\ StrMap.MapsTo "b"%string (2-bits of 0) (regState st)
-.
-Proof.
-  unfold evaluate_ndet.
-  eexists.
-  repeat split.
-  {
-    unfold nondeterminism1, initial_state; simpl.
-    eapply rt_trans.
-    - verilog_step_process_tac 2%positive.
-    - verilog_step_process_tac 1%positive.
-  }
-  all: simpl; simp eval_op bv_add_truncate.
-  - apply NameMap.is_empty_iff. reflexivity.
-  - apply StrMap.is_empty_iff. reflexivity.
-  - maps_to_tac.
-  - maps_to_tac.
-Qed.
+  Lemma final_is_blocked : forall st, final st -> blocked st.
+  Proof.
+    unfold final, blocked.
+    intros [reg procs] Hprocs.
+    simpl in *; subst.
+    simp step.
+    trivial.
+  Qed.
+End CombinationalOnly.
